KeyManagement/Common.v
@@ -1,0 +1,57 @@
+Require Import Frap.
+Set Implicit Arguments.
+
+
+Definition user_id              := nat.
+Definition user_list (A : Type) := list (user_id * A).
+
+Fixpoint updateUserList {V : Type} (usrs : user_list V) (u : user_id) (u_d : V) :=
+  match usrs with
+  | (k,v) :: usrs' => if k ==n u
+                     then (u,u_d) :: usrs' (* Case we are interested in *)
+                     else (k,v)   :: updateUserList usrs' u u_d
+  | []             => [(u,u_d)]
+  end.
+
+Theorem update_inserted:
+  forall V (users users' : user_list V) u_id v,
+    updateUserList users u_id v = users'
+    -> In (u_id,v) users'.
+Proof.
+  induct users; intros.
+  - unfold updateUserList in H. invert H. apply in_eq.
+  - destruct a. simpl in *. cases (u_id ==n u). simpl.
+    + rewrite e in *. rewrite <- H. cases (u ==n u); auto using in_eq. destruct n. trivial.
+    + cases (u ==n u_id).
+      * rewrite e in n. destruct n. trivial.
+      * destruct users'.
+        invert H.
+        apply in_cons. apply IHusers. inversion H. trivial.
+Qed.
+
+
+Print eq_nat_dec.
+
+Lemma pair_uneq_if_fst_uneq:
+  forall {A: Type} (p1 p2 : (user_id * A)) ineq,
+    ((fst p1) ==n (fst p2)) = right ineq
+    -> p1 <> p2.
+Proof.
+  intros. simpl. destruct p1 as [u1 a1]. destruct p2 as [u2 a2].
+  simpl in *. unfold not; intros. inversion H0. auto.
+Qed.
+
+Hint Resolve pair_uneq_if_fst_uneq.
+
+(* Theorem update_adds_no_duplicate_keys: *)
+(*   forall {V} (users users' : user_list V) u_id v, *)
+(*     (forall u_id1 u_id2 v1 v2, *)
+(*         In (u_id1,v1) users -> In (u_id2,v2) users -> u_id1 <> u_id2 \/ (u_id1 = u_id2 /\ v1 = v2)) *)
+(*     -> updateUserList users u_id v = users' *)
+(*     -> forall u_id1 u_id2 v1 v2, *)
+(*         In (u_id1,v1) users' -> In (u_id2,v2) users' -> u_id1 <> u_id2 \/ (u_id1 = u_id2 /\ v1 = v2). *)
+(* Proof. *)
+(*   induct users; intros; simpl in *; rewrite <- H0 in H1; rewrite <- H0 in H2. *)
+(*   - right. apply in_inv in H1; apply in_inv in H2. propositional; inversion H3; inversion H1; subst; auto. *)
+(*   - cases (u_id1 ==n u_id2). *)
+(*     + subst. destruct a. apply H; cases (u_id2 ==n u); right; subst; propositional. *)
