KeyManagement/RealWorld.v
@@ -1,0 +1,358 @@
+From Coq Require Import String.
+Require Import Frap.
+Require Import Common.
+
+Set Implicit Arguments.
+
+
+
+Definition key_identifier := nat.
+Definition cipher_id      := nat.
+
+Inductive key_usage :=
+| Encryption
+| Signing
+.
+
+Record cryptographic_key := MkCryptoKey {
+                                key_id : key_identifier ;
+                                usage  : key_usage
+                              }.
+
+(* A master key type *)
+Inductive key :=
+| SymKey   (k : cryptographic_key)
+| AsymKey  (k : cryptographic_key) (has_private_access : bool)
+.
+
+(** How are we going to model encryption / decryption in this framework?  Each key has
+    associated with it either:
+    - a key id (in the case of a symmetric key)
+    - a public/privite key pair (in the case of an asymmetric key)
+
+    In order for us to share a secret, we need to appropriately hide that secret so that
+    it cannot be viewed by eavesdroppers.  At the same time, for the purposes of this model
+    we are creating, we need to be able to detect very simply whether a decryption has been
+    successful.  The way we are going to do this, conceptually, is to include the key_id as
+    part of the message, and have the decryption step relation check whether that key_id
+    exists in the user's key heap.  Let's work out more precisely what happens in the two
+    cases:  symmetric and asymmetric keys.
+   
+    * Symmetric Key encryption / decryption
+
+    If I want to encrypt something and share it with someone else using a symmetric key, we
+    first have to generate the key and securely share it.  Ignoring things like usage and
+    the actual sharing process, the steps are:
+    - Generate symmetric key: private_key : symmetric_key := k (system adds to user's key heap)
+    - Securely share k (via Sym_Key_Msg, system adds to user's key heap)
+    - Sending user encrypts with k
+    - Sending user sends encrypted message to receiving user
+    - Receiving user decrypts with k (system verifies k is in decrypting user's key heap)
+
+    * Asymmetric Key encryption / decryption
+
+    Sharing a secret via asymmetric keys has a few more steps, but no 'magical' ones.  Each
+    user generates public/private key pairs, exchange the public parts, and encrypts with
+    a combination of own private key / destination user's public key.  The steps in more
+    detail:
+    - UserA generates key:
+        (pub_key_id, priv_key_id) : (nat,nat) := (pubIdA,privIdA)
+    - UserB generates key:
+        (pub_key_id, priv_key_id) : (nat,nat) := (pubIdB,privIdB)
+    - UserA publicly sends to UserB pubIdA
+    - UserB publicly sends to UserA pubIdB
+    - UserA encrypts message with pubIdB, sends to UserB
+    - UserB decrypts reeived message with privIdB
+ *)
+
+(* Messages ultimately wrap either a string or a key 
+   Messages can be encrypted, signed, or HMACed in a nested fashion any number of times 
+   Note: the key_pair_message constructor is temporary and will be removed *)
+Inductive message : Set -> Type :=
+(* Base Message Types *)
+| Plaintext {A : Set} (txt : A) : message A
+| KeyMessage  (k : key) : message key
+
+| MsgPair {A B : Set} (msg1 : message A) (msg2 : message B) : message (A*B)
+
+(* TODO tbraje: is there a way to collapse these two?? *)
+| Ciphertext (msg_id : cipher_id) : message cipher_id
+| Signature  (sig_id : cipher_id) : message cipher_id
+.
+
+Inductive user_cmd : Type -> Type :=
+(* Plumbing *)
+| Return {A : Type} (res : A) : user_cmd A
+| Bind {A A' : Type} (cmd1 : user_cmd A') (cmd2 : A' -> user_cmd A) : user_cmd A
+
+(* Messaging *)
+| Send {A : Set} (uid : user_id) (msg : message A) : user_cmd unit
+| Recv {A : Set}: user_cmd (message A)
+
+(* Crypto!! *)
+| Encrypt {A : Set} (k : key) (msg : message A) : user_cmd (message cipher_id)
+| Decrypt {A : Set} (msg : message cipher_id) : user_cmd (message A)
+
+| Sign    {A : Set} (k : key) (msg : message A) : user_cmd (message cipher_id)
+| Verify  (msg : message cipher_id) : user_cmd bool
+
+| GenerateSymKey  (usage : key_usage) : user_cmd key
+| GenerateAsymKey (usage : key_usage) : user_cmd key
+
+(* Allow administrator to make some global change to the universe -- revoke keys, etc. *)
+(* This may be a universe level step -- Administrator forces all users to stop *)
+(* | Barrier {result : Set} : user_cmd result *)
+.
+
+Notation "x <- c1 ; c2" := (Bind c1 (fun x => c2)) (right associativity, at level 75).
+
+(* Exisistential wrapper for message, so we can put it in collections *)
+(* This feels overly complicated to me... *) 
+Inductive exmsg : Type :=
+| Exm {A : Set} (msg : message A) : exmsg.
+
+Check ($0 $+ (1, Exm (Plaintext "foo")) $+ (2, Exm (Plaintext 1))).
+
+Record user_data (A : Type) :=
+  mkUserData {
+      usrid    : user_id ;
+      key_heap : fmap nat key ;
+      protocol : user_cmd A ;
+      (* msg_heap : user_msg_heap ; *)
+      (* is_admin : bool *)
+    }.
+
+Inductive cipher : Type :=
+| Cipher {A: Set} (c_id : cipher_id) (k_id : key_identifier) (msg : message A) : cipher
+.
+
+Definition queued_messages := fmap user_id (list exmsg).
+Definition keys            := fmap key_identifier key.
+Definition ciphers         := fmap cipher_id cipher.
+
+Record universe (A : Type) :=
+  mkUniverse {
+      users            : user_list (user_data A) ;
+      users_msg_buffer : queued_messages ;
+      all_keys         : keys ;
+      all_ciphers      : ciphers
+    }.
+
+(* This is horribly inefficient, but I want the list to act like a queue.  We want
+ * first in - first out semantics to keep message order preserved *)
+Local Definition multiMapAdd {K V} (k : K)(v : V)(m : fmap K (list V)) : fmap K (list V) :=
+  match m $? k with
+  | None => m $+ (k, [v])
+  | Some vs => m $+ (k, vs ++ [v]) (* add new element to end, to preserve order *)
+  end.
+
+(* When we are finding keys, we need to check whether they are asymmetric.  If
+   so, we mark them as not having access to the private key, since the intent is to
+   send only the public part of the key *)
+Local Fixpoint findKeys {A} (msg : message A) : list key :=
+  match msg with
+  | Plaintext pt       => []
+
+  | KeyMessage (AsymKey k' _) => [AsymKey k' false] (* Only sending public keys *)
+  | KeyMessage k       => [k]
+  | MsgPair msg1 msg2  => findKeys msg1 ++ findKeys msg2
+  | Ciphertext _       => []
+  | Signature _        => []
+  end.
+
+Local Definition updateKeyHeap (ks : list key) (key_heap : keys) : keys :=
+  let addKey (m : keys) (k : key) :=
+      match k with
+      | SymKey k'     => m $+ (k'.(key_id), k)
+      | AsymKey k' b  => m $+ (k'.(key_id), k)
+      end
+  in  fold_left addKey ks key_heap.
+
+Local Definition updateUserKeyHeap {A : Set} (ks : list key) (ud : user_data A) : user_data A :=
+  {| usrid    := ud.(usrid)
+     ; key_heap := updateKeyHeap ks ud.(key_heap)
+     ; protocol := ud.(protocol)
+  |}.
+
+Definition encryptMessage {A} (k : key) (m : message A) (c_id : cipher_id) : option cipher :=
+  match k with
+  | SymKey k'  =>
+    match (usage k') with
+    | Encryption => Some (Cipher c_id k'.(key_id) m)
+    | _          => None
+    end
+  | AsymKey k' _ => (* Encryption always uses the public part of an asymmetric key *)
+    match (usage k') with
+    | Encryption => Some (Cipher c_id k'.(key_id) m)
+    | _          => None
+    end
+  end.
+
+Definition signMessage {A} (k : key) (m : message A) (c_id : cipher_id) : option cipher :=
+  match k with
+  | SymKey k'  =>
+    match (usage k') with
+    | Signing => Some (Cipher c_id k'.(key_id) m)
+    | _       => None
+    end
+  | AsymKey k' true => (* Signing requires private key, so check we have access *)
+    match (usage k') with
+    | Signing => Some (Cipher c_id k'.(key_id) m)
+    | _       => None
+    end
+  | _ => None
+  end.
+
+Definition canVerifySignature {A} (ciphers : fmap cipher_id cipher)(usrDat : user_data A)(c_id : cipher_id) : Prop :=
+  forall {A} (m : message A) k_id k ,
+    ciphers $? c_id = Some (Cipher c_id k_id m)
+    (*  Make sure that the user has access to the key.  If we are doing asymmetric signatures,
+        we only need the public part of the key, so no additional checks necessary! *)
+    /\ usrDat.(key_heap) $? k_id = Some k.
+
+Definition data_step0 (A : Type) : Type := 
+  ciphers * keys * queued_messages * fmap nat key * user_cmd A.
+
+Inductive step_user : forall A, user_id -> data_step0 A -> data_step0 A -> Prop :=
+
+(* Plumbing *)
+| StepBindRecur : forall {r r'} u_id cs cs' ks ks' msgs msgs' uks uks' (cmd1 cmd1' : user_cmd r) (cmd2 : r -> user_cmd r'),
+    step_user u_id (cs, ks, msgs, uks, cmd1) (cs', ks', msgs', uks', cmd1')
+    -> step_user u_id (cs, ks, msgs, uks, Bind cmd1 cmd2) (cs', ks', msgs', uks', Bind cmd1' cmd2)
+| StepBindProceed : forall {r r'} u_id cs ks msgs uks (v : r') (cmd : r' -> user_cmd r),
+    step_user u_id (cs, ks, msgs, uks, Bind (Return v) cmd) (cs, ks, msgs, uks, cmd v)
+
+(* Comms *)
+| StepRecv : forall {A} u_id cs ks qmsgs uks (msg : message A) msgs newkeys,
+    qmsgs $? u_id = Some (Exm msg :: msgs) (* we have a message waiting for us! *)
+    -> findKeys msg = newkeys
+    -> step_user u_id (cs, ks, qmsgs, uks, Recv)
+                     (cs, ks, qmsgs $+ (u_id, msgs), updateKeyHeap newkeys uks, Return msg)
+| StepSend : forall {A} u_id cs ks qmsgs rec_u_id uks (msg : message A),
+    step_user u_id (cs, ks, qmsgs, uks, Send rec_u_id msg)
+                   (cs, ks, multiMapAdd rec_u_id (Exm msg) qmsgs, uks, Return tt)
+
+(* Encryption / Decryption *)
+(* | StepEncrypt : forall {A} cs ks qmsgs usrDat (msg : message A) k k_id c_id cipherMsg, *)
+(*     usrDat.(key_heap) $? k_id = Some k *)
+(*     -> ~(c_id \in (dom cs)) *)
+(*     -> encryptMessage k msg c_id = Some cipherMsg *)
+(*     -> step_user (cs, ks, qmsgs, usrDat, Encrypt k msg) *)
+(*                 (cs $+ (c_id, cipherMsg), ks, qmsgs, usrDat, Return (Ciphertext c_id)) *)
+
+(* | StepSymmetricDecrypt : forall {A} cs ks qmsgs usrDat (msg : message A) k_id k c_id newkeys, *)
+(*     cs $? c_id = Some (Cipher c_id k_id msg) *)
+(*     -> usrDat.(key_heap) $? k_id = Some (SymKey k) *)
+(*     -> findKeys msg = newkeys (* find keys in new key heap *) *)
+(*     -> step_user (cs, ks, qmsgs, usrDat, Decrypt (Ciphertext c_id)) *)
+(*                 (cs, ks, qmsgs, updateUserKeyHeap newkeys usrDat, Return msg) *)
+
+(* | StepAsymmetricDecrypt : forall {A} cs ks qmsgs usrDat (msg : message A) k_id k c_id newkeys, *)
+(*     cs $? c_id = Some (Cipher c_id k_id msg) *)
+(*     -> usrDat.(key_heap) $? k_id = Some (AsymKey k true) (* check we have access to private key *) *)
+(*     -> findKeys msg = newkeys *)
+(*     -> step_user (cs, ks, qmsgs, usrDat, Decrypt (Ciphertext c_id)) *)
+(*                 (cs, ks, qmsgs, updateUserKeyHeap newkeys usrDat, Return msg) *)
+
+(* Signing / Verification *)
+(* | StepSign : forall {A} cs ks qmsgs usrDat k_id k (msg : message A) c_id cipherMsg, *)
+(*     usrDat.(key_heap) $? k_id = Some k *)
+(*     -> ~(c_id \in (dom cs)) *)
+(*     -> signMessage k msg c_id = Some cipherMsg *)
+(*     -> step_user (cs, ks, qmsgs, usrDat, Sign k msg) *)
+(*                 (cs $+ (c_id, cipherMsg), ks, qmsgs, usrDat, Return (Signature c_id)) *)
+(* | StepVerify : forall cs ks qmsgs usrDat c_id, *)
+(*     canVerifySignature cs usrDat c_id *)
+(*     -> step_user (cs, ks, qmsgs, usrDat, Verify (Signature c_id)) *)
+(*                 (cs, ks, qmsgs, usrDat, Return true) *)
+(* | StepFailVerify : forall cs ks qmsgs usrDat c_id, *)
+(*     ~ canVerifySignature cs usrDat c_id *)
+(*     -> step_user (cs, ks, qmsgs, usrDat, Verify (Signature c_id)) *)
+(*                 (cs, ks, qmsgs, usrDat, Return false) *)
+(* | StepFailVerifyNotSig : forall cs ks qmsgs usrDat c_id msg, *)
+(*     ~ msg <> Signature c_id *)
+(*     -> step_user (cs, ks, qmsgs, usrDat, Verify msg) *)
+(*                 (cs, ks, qmsgs, usrDat, Return false) *)
+
+(* Key creation *)
+(* | StepGenerateSymKey: forall A cs ks qmsgs (usrDat : user_data A) usage k kid, *)
+(*     ~(kid \in (dom ks)) *)
+(*     -> k = SymKey (MkCryptoKey kid usage) *)
+(*     -> step_user (cs, ks, qmsgs, usrDat, GenerateSymKey usage) *)
+(*                 (cs, ks $+ (kid, k), qmsgs, updateUserKeyHeap [k] usrDat, Return k) *)
+(* | StepGenerateAsymKey: forall {a : Set} cs ks qmsgs (usrDat : user_data a) usage k kid, *)
+(*     ~(kid \in (dom ks)) *)
+(*     -> k = AsymKey (MkCryptoKey kid usage) true *)
+(*     -> step_user (cs, ks, qmsgs, usrDat, GenerateAsymKey usage) *)
+(*                 (cs, ks $+ (kid, k), qmsgs, updateUserKeyHeap [k] usrDat, Return k) *)
+                
+(* | Barrier {result : Set} : user_cmd result. *)
+.
+
+Definition updateUniverse {A} (U : universe A) (cs : ciphers) (ks : keys) (qmsgs : queued_messages)
+                          (u_id : user_id) (userKeys : keys) (cmd : user_cmd A): universe A :=
+  {|
+    users            := updateUserList U.(users) u_id ( mkUserData u_id userKeys cmd )
+  ; users_msg_buffer := qmsgs
+  ; all_keys         := ks
+  ; all_ciphers      := cs
+  |}.
+
+Inductive step_universe {A} : universe A -> universe A -> Prop :=
+| StepUser : forall U u_id userData uks cs ks qmsgs (cmd cmd' : user_cmd A),
+    In (u_id,userData) U.(users)
+    (* U.(users) $? u_id = Some userData *)
+    -> step_user u_id (U.(all_ciphers), U.(all_keys), U.(users_msg_buffer), userData.(key_heap), cmd)
+                     (cs, ks, qmsgs, uks, cmd')
+    -> step_universe U (updateUniverse U cs ks qmsgs u_id uks cmd')
+.
+
+Definition extractPlainText {A} (msg : message A) : option A :=
+  match msg with
+  | Plaintext t => Some t
+  | _           => None
+  end.
+
+
+
+Section PingProtocol.
+
+  Example ping : list (user_data nat) :=
+    {| usrid    := 0
+     ; key_heap := $0
+     ; protocol := (  _ <- Send 1 (Plaintext 1)
+                    ; rec <- Recv (A := nat)
+                    ; Return (match extractPlainText rec with
+                              | (Some msg) => msg
+                              | None       => 99
+                              end))
+    |}
+      ::
+    {| usrid    := 1
+     ; key_heap := $0
+     ; protocol := (  rec <- Recv (A := nat)
+                    ; _ <- Send 0 (Plaintext 0)
+                    ; Return (match extractPlainText rec with
+                              | Some msg => msg
+                              | None     => 98
+                              end))
+    |}
+      :: [].
+
+  Example ping_universe : universe nat :=
+    {|
+      users            := map (fun u_d => (u_d.(usrid), u_d)) ping
+    ; users_msg_buffer := $0
+    ; all_keys         := $0
+    ; all_ciphers      := $0
+    |}.
+
+  Check ping_universe.
+
+End PingProtocol.
+
+
+(* Additional functionality to implement:
+   1. Administration
+   2. CA
+*) 
