KeyManagement/Simulation.v
@@ -1,0 +1,115 @@
+(* From Coq Require Import Basics. *)
+Require Import Frap.
+
+Require Import Common.
+Require IdealWorld.
+Require RealWorld.
+
+Set Implicit Arguments.
+
+
+
+Definition idealWorldIsReallyFinalState {A} (U : IdealWorld.universe A) : Prop :=
+  Forall (fun '(_,prog) => exists a, prog = IdealWorld.Return a) U.(IdealWorld.users).
+
+Definition realWorldIsReallyFinalState {A} (U : RealWorld.universe A) : Prop :=
+  Forall (fun '(_,u_data) => exists a, u_data.(RealWorld.protocol) = RealWorld.Return a) U.(RealWorld.users).
+
+Definition idealWorldReturnOf {A} (c : IdealWorld.cmd A) : option A :=
+  match c with
+  | IdealWorld.Return a => Some a
+  | _                   => None
+  end.
+
+Definition realWorldReturnOf {A} (c : RealWorld.user_data A) : option A :=
+  match c.(RealWorld.protocol) with
+  | RealWorld.Return a => Some a
+  | _                  => None
+  end.
+
+Fixpoint returnsOfHelper {B : Type} {A : Type -> Type} (users : user_list (A B)) (f : A B -> option B) : list B :=
+  match users with
+  | []          => []
+  | (_,a) :: xs =>
+    match f a with
+    | Some b => b :: returnsOfHelper xs f
+    | None   => returnsOfHelper xs f
+    end
+  end.
+
+(* Fixpoint idealWorldReturnsOf' {A} (users : user_list (IdealWorld.cmd A)) : list A := *)
+(*   match users with *)
+(*   | []      => [] *)
+(*   | (_,c) :: xs => *)
+(*     match idealWorldReturnOf c with *)
+(*     | Some a => a :: idealWorldReturnsOf' xs *)
+(*     | None   => idealWorldReturnsOf' xs *)
+(*     end *)
+(*     (* match c in (IdealWorld.cmd A') return (list A' -> list A') with *) *)
+(*     (* | IdealWorld.Return a => fun xs => a :: xs *) *)
+(*     (* | _                   => fun xs => xs *) *)
+(*     (* end (idealWorldReturnsOf' xs) *) *)
+(*   end. *)
+
+Definition idealWorldReturnsOf {A : Type} (U : IdealWorld.universe A) : list A :=
+  returnsOfHelper U.(IdealWorld.users) idealWorldReturnOf.
+
+Definition realWorldReturnsOf {A : Type} (U : RealWorld.universe A) : list A :=
+  returnsOfHelper U.(RealWorld.users) realWorldReturnOf.
+
+
+
+Definition finalAnswerInclusion {A} (U1 : IdealWorld.universe A) (U2 : RealWorld.universe A) :=
+
+  forall finalStateOfU1, IdealWorld.step_universe^* U1 finalStateOfU1
+                    -> idealWorldIsReallyFinalState finalStateOfU1
+                    -> exists finalStateOfU2, RealWorld.step_universe^* U2 finalStateOfU2
+                                        /\ realWorldIsReallyFinalState finalStateOfU2
+                                        /\ idealWorldReturnsOf finalStateOfU1 = realWorldReturnsOf finalStateOfU2.
+
+
+
+
+
+
+
+(* multi step relation for some users in U1 *)
+
+
+
+
+Definition stepSilent (U1 U2 : u)   := step_universe U1 Silent U2.
+Definition kstepSilent (U1 U2 : ku) := Keys.step_universe U1 Keys.Silent U2.
+
+Inductive actionCorrespondance : observable -> Keys.Observable -> Prop :=
+| EqSendPlain : forall {A : Set} o ko usr1 usr2 (msg1 : A) (msg2 : Keys.message A),
+    o = Output usr1 msg1
+    -> ko = Keys.Output usr2 msg2
+    (* Something here about equality of messages and users.
+     * Will eventually need to handle the notion of encryption! *)
+    -> msg2 = Keys.Plaintext msg1 (* sending the same body!! *)
+    -> actionCorrespondance o ko.
+ 
+Definition simulates (R : u -> ku -> Prop) (U : u) (KU : ku) :=
+  (forall U KU, R U KU
+           -> forall U', stepSilent U U'
+                   -> exists KU', kstepSilent^* KU KU'
+                            /\ R U' KU')
+
+  /\ (forall U KU, R U KU
+             -> forall a1 a2 U', step_universe U (Visible a1) U'
+                       -> exists KU' KU'', kstepSilent^* KU KU'
+                                     /\ Keys.step_universe KU' (Keys.Visible a2) KU''
+                                     (* We may eventually need here to handle multiple
+                                      * real world steps in order to collect the things
+                                      * needed to ensure the same cryptographic properties
+                                      * hold between the two universes *)
+                                     /\ actionCorrespondance a1 a2
+                                     /\ R U' KU'')
+  
+
+  /\ R U KU.
+
+Definition refines (U1 : u) (U2 : ku) :=
+  exists R, simulates R U1 U2.
+
