Makefile
@@ -1,0 +1,16 @@
+.PHONY: all coq frap
+
+all: coq
+
+frap:
+	$(MAKE) -C frap
+
+coq: Makefile.coq frap
+	$(MAKE) -f Makefile.coq
+
+Makefile.coq: Makefile _CoqProject
+	coq_makefile -f _CoqProject -o Makefile.coq
+
+clean:: Makefile.coq
+	$(MAKE) -f Makefile.coq clean
+	rm -f Makefile.coq
